James C - started chapter 20

isabelle/Chapter20_1_Language.thy
@@ -1,304 +1,102 @@
 theory Chapter20_1_Language
-imports AssocList DeBruijn
+imports DeBruijnEnvironment
 begin
 
 datatype type = 
-  Arr type type 
-| Unit 
-| Prod type type 
-| Void 
-| Sum type type
-| Tyvar nat
-| Rec type
+  Tyvar var
+| Nat
+| Arrow type type
 | All type
-
-primrec is_valid_type :: "nat set => type => bool"
-where "is_valid_type tyvars (Arr t1 t2) = (is_valid_type tyvars t1 & is_valid_type tyvars t2)"
-    | "is_valid_type tyvars Unit = True"
-    | "is_valid_type tyvars (Prod t1 t2) = (is_valid_type tyvars t1 & is_valid_type tyvars t2)"
-    | "is_valid_type tyvars Void = True"
-    | "is_valid_type tyvars (Sum t1 t2) = (is_valid_type tyvars t1 & is_valid_type tyvars t2)"
-    | "is_valid_type tyvars (Tyvar v) = (v : tyvars)"
-    | "is_valid_type tyvars (Rec t) = is_valid_type (expand_set tyvars) t"
-    | "is_valid_type tyvars (All t) = is_valid_type (expand_set tyvars) t"
-
-primrec type_free_vars :: "type => nat set"
-where "type_free_vars (Tyvar v) = {v}"
-    | "type_free_vars (Arr e1 e2) = type_free_vars e1 Un type_free_vars e2"
-    | "type_free_vars Unit = {}"
-    | "type_free_vars (Prod e1 e2) = type_free_vars e1 Un type_free_vars e2"
-    | "type_free_vars Void = {}"
-    | "type_free_vars (Sum e1 e2) = type_free_vars e1 Un type_free_vars e2"
-    | "type_free_vars (Rec t) = redr_set (type_free_vars t)"
-    | "type_free_vars (All t) = redr_set (type_free_vars t)"
-
-primrec type_sub_from :: "nat => type => type"
-where "type_sub_from n (Tyvar v) = Tyvar (subr n v)"
-    | "type_sub_from n (Arr e1 e2) = Arr (type_sub_from n e1) (type_sub_from n e2)"
-    | "type_sub_from n Unit = Unit"
-    | "type_sub_from n (Prod e1 e2) = Prod (type_sub_from n e1) (type_sub_from n e2)"
-    | "type_sub_from n Void = Void"
-    | "type_sub_from n (Sum e1 e2) = Sum (type_sub_from n e1) (type_sub_from n e2)"
-    | "type_sub_from n (Rec t) = Rec (type_sub_from (Suc n) t)"
-    | "type_sub_from n (All t) = All (type_sub_from (Suc n) t)"
-
-primrec type_incr_from :: "nat => type => type"
-where "type_incr_from n (Tyvar v) = Tyvar (incr n v)"
-    | "type_incr_from n (Arr e1 e2) = Arr (type_incr_from n e1) (type_incr_from n e2)"
-    | "type_incr_from n Unit = Unit"
-    | "type_incr_from n (Prod e1 e2) = Prod (type_incr_from n e1) (type_incr_from n e2)"
-    | "type_incr_from n Void = Void"
-    | "type_incr_from n (Sum e1 e2) = Sum (type_incr_from n e1) (type_incr_from n e2)"
-    | "type_incr_from n (Rec t) = Rec (type_incr_from (Suc n) t)"
-    | "type_incr_from n (All t) = All (type_incr_from (Suc n) t)"
-
-primrec type_subst' :: "type => type => nat => type"
-where "type_subst' (Tyvar v) t x = (if v = x then t else Tyvar v)"
-    | "type_subst' (Arr t1 t2) t x = Arr (type_subst' t1 t x) (type_subst' t2 t x)"
-    | "type_subst' Unit t x = Unit"
-    | "type_subst' (Prod t1 t2) t x = Prod (type_subst' t1 t x) (type_subst' t2 t x)"
-    | "type_subst' Void t x = Void"
-    | "type_subst' (Sum t1 t2) t x = Sum (type_subst' t1 t x) (type_subst' t2 t x)"
-    | "type_subst' (Rec t0) t x = Rec (type_subst' t0 (type_incr_from 0 t) (Suc x))"
-    | "type_subst' (All t0) t x = All (type_subst' t0 (type_incr_from 0 t) (Suc x))"
-
-definition type_subst :: "type => type => type"
-where "type_subst e e' = type_sub_from 0 (type_subst' e (type_incr_from 0 e') 0)"
-
-lemma [simp]: "type_free_vars (type_incr_from n e) = incr n ` type_free_vars e"
-by (induction e arbitrary: n, auto)
-
-lemma valid_incr_type [simp]: "is_valid_type (expand_set_at m s) (type_incr_from m t) = is_valid_type s t"
-by (induction t arbitrary: s m, simp_all)
-
-lemma [simp]: "is_valid_type (expand_set s) (type_incr_from 0 t) = is_valid_type s t"
-proof -
-  from valid_incr_type have X: "is_valid_type (expand_set_at 0 s) (type_incr_from 0 t) = is_valid_type s t" by presburger
-  have "expand_set_at 0 s = expand_set s" by simp
-  with X show "is_valid_type (expand_set s) (type_incr_from 0 t) = is_valid_type s t" by simp
-qed
-
-lemma [simp]: "m < n ==> type_incr_from m (type_sub_from n t) = type_sub_from (Suc n) (type_incr_from m t)"
-by (induction t arbitrary: n m, simp_all)
-
-lemma [simp]: "type_sub_from n (type_incr_from n t) = t"
-by (induction t arbitrary: n, simp_all)
-
-lemma [simp]: "m <= n ==> type_incr_from m (type_incr_from n t) = type_incr_from (Suc n) (type_incr_from m t)"
-by (induction t arbitrary: n m, simp_all)
-
-lemma [simp]: "type_incr_from m (type_subst' a t x) = type_subst' (type_incr_from m a) (type_incr_from m t) (incr m x)"
-by (induction a arbitrary: t x m, auto simp add: incr_def)
-
-primrec type_incr_by :: "nat => type => type"
-where "type_incr_by 0 e = e"
-    | "type_incr_by (Suc n) e = type_incr_from 0 (type_incr_by n e)"
-
-lemma [simp]:  "redr_set_by n (type_free_vars (type_incr_by n e)) = type_free_vars e" 
-by (induction n, simp_all) 
-
-lemma [simp]: "type_free_vars (type_subst' e e' x) = (if x : type_free_vars e then type_free_vars e - {x} Un type_free_vars e' else type_free_vars e)"
-by (induction e arbitrary: e' x, auto)
+| Unit
+| Prod type type
+| Void
+| Sum type type
 
 datatype expr = 
-  Var nat 
+  Var var
+| Zero
+| Suc expr
+| Rec expr expr expr
 | Lam type expr
-| Ap expr expr
-| Fix type expr
+| Appl expr expr
+| TyLam expr
+| TyAppl type expr
 | Triv
 | Pair expr expr
 | ProjL expr
 | ProjR expr
 | Abort type expr
+| Case expr expr expr
 | InL type type expr
 | InR type type expr
-| Case expr expr expr
-| Fold type expr
-| Unfold expr
-| TyLam expr
-| TyAp type expr
 
-primrec free_vars :: "expr => nat set"
-where "free_vars (Var v) = {v}"
-    | "free_vars (Lam t b) = redr_set (free_vars b)"
-    | "free_vars (Ap e1 e2) = free_vars e1 Un free_vars e2"
-    | "free_vars (Fix t b) = redr_set (free_vars b)"
-    | "free_vars Triv = {}"
-    | "free_vars (Pair e1 e2) = free_vars e1 Un free_vars e2"
-    | "free_vars (ProjL e) = free_vars e"
-    | "free_vars (ProjR e) = free_vars e"
-    | "free_vars (Abort t e) = free_vars e"
-    | "free_vars (InL t t' e) = free_vars e"
-    | "free_vars (InR t t' e) = free_vars e"
-    | "free_vars (Case e el er) = free_vars e Un redr_set (free_vars el) Un redr_set (free_vars er)"
-    | "free_vars (Fold t e) = free_vars e"
-    | "free_vars (Unfold e) = free_vars e"
-    | "free_vars (TyLam e) = free_vars e"
-    | "free_vars (TyAp t e) = free_vars e"
+primrec insert :: "var => expr => expr"
+where "insert n (Var v) = Var (incr n v)"
+    | "insert n Zero = Zero"
+    | "insert n (Suc e) = Suc (insert n e)"
+    | "insert n (Rec et e0 es) = Rec (insert n et) (insert n e0) (insert (next (next n)) es)"
+    | "insert n (Lam t e) = Lam t (insert (next n) e)"
+    | "insert n (Appl e1 e2) = Appl (insert n e1) (insert n e2)"
+    | "insert n (TyLam e) = TyLam (insert n e)"
+    | "insert n (TyAppl t e) = TyAppl t (insert n e)"
+    | "insert n Triv = Triv"
+    | "insert n (Pair e1 e2) = Pair (insert n e1) (insert n e2)"
+    | "insert n (ProjL e) = ProjL (insert n e)"
+    | "insert n (ProjR e) = ProjR (insert n e)"
+    | "insert n (Abort t e) = Abort t (insert n e)"
+    | "insert n (Case et el er) = Case (insert n et) (insert (next n) el) (insert (next n) er)"
+    | "insert n (InL t1 t2 e) = InL t1 t2 (insert n e)"
+    | "insert n (InR t1 t2 e) = InR t1 t2 (insert n e)"
 
-primrec incr_from :: "nat => expr => expr"
-where "incr_from n (Var v) = Var (incr n v)"
-    | "incr_from n (Lam t b) = Lam t (incr_from (Suc n) b)"
-    | "incr_from n (Ap e1 e2) = Ap (incr_from n e1) (incr_from n e2)"
-    | "incr_from n (Fix t b) = Fix t (incr_from (Suc n) b)"
-    | "incr_from n Triv = Triv"
-    | "incr_from n (Pair e1 e2) = Pair (incr_from n e1) (incr_from n e2)"
-    | "incr_from n (ProjL e) = ProjL (incr_from n e)"
-    | "incr_from n (ProjR e) = ProjR (incr_from n e)"
-    | "incr_from n (Abort t e) = Abort t (incr_from n e)"
-    | "incr_from n (InL t t' e) = InL t t' (incr_from n e)"
-    | "incr_from n (InR t t' e) = InR t t' (incr_from n e)"
-    | "incr_from n (Case e el er) = Case (incr_from n e) (incr_from (Suc n) el) (incr_from (Suc n) er)"
-    | "incr_from n (Fold t e) = Fold t (incr_from n e)"
-    | "incr_from n (Unfold e) = Unfold (incr_from n e)"
-    | "incr_from n (TyLam e) = TyLam (incr_from n e)"
-    | "incr_from n (TyAp t e) = TyAp t (incr_from n e)"
+primrec remove :: "var => expr => expr"
+where "remove n (Var v) = Var (subr n v)"
+    | "remove n Zero = Zero"
+    | "remove n (Suc e) = Suc (remove n e)"
+    | "remove n (Rec et e0 es) = Rec (remove n et) (remove n e0) (remove (next (next n)) es)"
+    | "remove n (Lam t e) = Lam t (remove (next n) e)"
+    | "remove n (Appl e1 e2) = Appl (remove n e1) (remove n e2)"
+    | "remove n (TyLam e) = TyLam (remove n e)"
+    | "remove n (TyAppl t e) = TyAppl t (remove n e)"
+    | "remove n Triv = Triv"
+    | "remove n (Pair e1 e2) = Pair (remove n e1) (remove n e2)"
+    | "remove n (ProjL e) = ProjL (remove n e)"
+    | "remove n (ProjR e) = ProjR (remove n e)"
+    | "remove n (Abort t e) = Abort t (remove n e)"
+    | "remove n (Case et el er) = Case (remove n et) (remove (next n) el) (remove (next n) er)"
+    | "remove n (InL t1 t2 e) = InL t1 t2 (remove n e)"
+    | "remove n (InR t1 t2 e) = InR t1 t2 (remove n e)"
 
-primrec sub_from :: "nat => expr => expr"
-where "sub_from n (Var v) = Var (if v < n then v else v - 1)"
-    | "sub_from n (Lam t b) = Lam t (sub_from (Suc n) b)"
-    | "sub_from n (Ap e1 e2) = Ap (sub_from n e1) (sub_from n e2)"
-    | "sub_from n (Fix t b) = Fix t (sub_from (Suc n) b)"
-    | "sub_from n Triv = Triv"
-    | "sub_from n (Pair e1 e2) = Pair (sub_from n e1) (sub_from n e2)"
-    | "sub_from n (ProjL e) = ProjL (sub_from n e)"
-    | "sub_from n (ProjR e) = ProjR (sub_from n e)"
-    | "sub_from n (Abort t e) = Abort t (sub_from n e)"
-    | "sub_from n (InL t t' e) = InL t t' (sub_from n e)"
-    | "sub_from n (InR t t' e) = InR t t' (sub_from n e)"
-    | "sub_from n (Case e el er) = Case (sub_from n e) (sub_from (Suc n) el) (sub_from (Suc n) er)"
-    | "sub_from n (Fold t e) = Fold t (sub_from n e)"
-    | "sub_from n (Unfold e) = Unfold (sub_from n e)"
-    | "sub_from n (TyLam e) = TyLam (sub_from n e)"
-    | "sub_from n (TyAp t e) = TyAp t (sub_from n e)"
-
-primrec subst' :: "expr => expr => nat => expr"
-where "subst' (Var v) e x = (if v = x then e else Var v)"
-    | "subst' (Lam t b) e x = Lam t (subst' b (incr_from 0 e) (Suc x))"
-    | "subst' (Ap e1 e2) e x = Ap (subst' e1 e x) (subst' e2 e x)"
-    | "subst' (Fix t b) e x = Fix t (subst' b (incr_from 0 e) (Suc x))"
-    | "subst' Triv e x = Triv"
-    | "subst' (Pair e1 e2) e x = Pair (subst' e1 e x) (subst' e2 e x)"
-    | "subst' (ProjL n) e x = ProjL (subst' n e x)"
-    | "subst' (ProjR n) e x = ProjR (subst' n e x)"
-    | "subst' (Abort t n) e x = Abort t (subst' n e x)"
-    | "subst' (InL t t' n) e x = InL t t' (subst' n e x)"
-    | "subst' (InR t t' n) e x = InR t t' (subst' n e x)"
-    | "subst' (Case n el er) e x = Case (subst' n e x) (subst' el (incr_from 0 e) (Suc x)) (subst' er (incr_from 0 e) (Suc x))"
-    | "subst' (Fold t n) e x = Fold t (subst' n e x)"
-    | "subst' (Unfold n) e x = Unfold (subst' n e x)"
-    | "subst' (TyLam n) e x = TyLam (subst' n e x)"
-    | "subst' (TyAp t n) e x = TyAp t (subst' n e x)"
+primrec subst' :: "var => expr => expr => expr"
+where "subst' n e' (Var v) = (if v = n then e' else Var v)"
+    | "subst' n e' Zero = Zero"
+    | "subst' n e' (Suc e) = Suc (subst' n e' e)"
+    | "subst' n e' (Rec et e0 es) = 
+                      Rec (subst' n e' et) 
+                          (subst' n e' e0) 
+                          (subst' (next (next n)) (insert first (insert first e')) es)"
+    | "subst' n e' (Lam t e) = Lam t (subst' (next n) (insert first e') e)"
+    | "subst' n e' (Appl e1 e2) = Appl (subst' n e' e1) (subst' n e' e2)"
+    | "subst' n e' (TyLam e) = TyLam (subst' n e' e)"
+    | "subst' n e' (TyAppl t e) = TyAppl t (subst' n e' e)"
+    | "subst' n e' Triv = Triv"
+    | "subst' n e' (Pair e1 e2) = Pair (subst' n e' e1) (subst' n e' e2)"
+    | "subst' n e' (ProjL e) = ProjL (subst' n e' e)"
+    | "subst' n e' (ProjR e) = ProjR (subst' n e' e)"
+    | "subst' n e' (Abort t e) = Abort t (subst' n e' e)"
+    | "subst' n e' (Case et el er) = 
+                      Case (subst' n e' et) 
+                           (subst' (next n) (insert first e') el) 
+                           (subst' (next n) (insert first e') er)"
+    | "subst' n e' (InL t1 t2 e) = InL t1 t2 (subst' n e' e)"
+    | "subst' n e' (InR t1 t2 e) = InR t1 t2 (subst' n e' e)"
 
 definition subst :: "expr => expr => expr"
-where "subst e e' = sub_from 0 (subst' e (incr_from 0 e') 0)"
+where "subst e' e = remove first (subst' first (insert first e') e)"
 
-lemma [simp]: "free_vars (incr_from n e) = incr n ` free_vars e"
-by (induction e arbitrary: n, auto)
+lemma [simp]: "remove n (insert n e) = e"
+by (induction e arbitrary: n, simp_all)
 
-primrec incr_by :: "nat => expr => expr"
-where "incr_by 0 e = e"
-    | "incr_by (Suc n) e = incr_from 0 (incr_by n e)"
-
-lemma [simp]:  "redr_set_by n (free_vars (incr_by n e)) = free_vars e" 
-by (induction n, simp_all) 
-
-lemma [simp]: "free_vars (subst' e e' x) = (if x : free_vars e then free_vars e - {x} Un free_vars e' else free_vars e)"
-by (induction e arbitrary: e' x, auto)
-
-lemma [simp]: "m <= n ==> incr_from (Suc n) (incr_from m e) = incr_from m (incr_from n e)"
-by (induction e arbitrary: m n, simp_all add: incr_def)
-
-lemma [simp]: "m <= n ==> n ~: free_vars e ==> sub_from (Suc n) (incr_from m e) = incr_from m (sub_from n e)"
-by (induction e arbitrary: n m, auto simp add: incr_def)
-
-lemma [simp]: "sub_from n (incr_from n e) = e"
-by (induction e arbitrary: n, auto simp add: incr_def)
-
-lemma [simp]: "m <= x ==> subst' (incr_from m e) (incr_from m e') (Suc x) = incr_from m (subst' e e' x)"
-proof (induction e arbitrary: m e' x) 
-case (Var v) 
-  thus ?case by (simp add: incr_def)
-next case (Lam t b) 
-  hence "subst' (incr_from (Suc m) b) (incr_from (Suc m) (incr_from 0 e')) (Suc (Suc x)) = incr_from (Suc m) (subst' b (incr_from 0 e') (Suc x))" by blast 
-  thus ?case by simp
-next case (Ap e1 e2) 
-  thus ?case by simp
-next case (Fix t b) 
-  hence "subst' (incr_from (Suc m) b) (incr_from (Suc m) (incr_from 0 e')) (Suc (Suc x)) = incr_from (Suc m) (subst' b (incr_from 0 e') (Suc x))" by blast
-  thus ?case by simp
-next case Triv 
-  thus ?case by simp
-next case (Pair e1 e2) 
-  thus ?case by simp
-next case (ProjL e) 
-  thus ?case by simp
-next case (ProjR e) 
-  thus ?case by simp
-next case (Abort t e) 
-  thus ?case by simp
-next case (InL t t' e) 
-  thus ?case by simp
-next case (InR t t' e) 
-  thus ?case by simp
-next case (Case e el er) 
-  from Case have "subst' (incr_from m e) (incr_from m e') (Suc x) = incr_from m (subst' e e' x)" by blast
-  moreover from Case have "subst' (incr_from (Suc m) el) (incr_from (Suc m) (incr_from 0 e')) (Suc (Suc x)) = incr_from (Suc m) (subst' el (incr_from 0 e') (Suc x))" by blast
-  moreover from Case have "subst' (incr_from (Suc m) er) (incr_from (Suc m) (incr_from 0 e')) (Suc (Suc x)) = incr_from (Suc m) (subst' er (incr_from 0 e') (Suc x))" by (metis Suc_le_mono)
-  ultimately show ?case by simp
-next case (Fold t e) 
-  thus ?case by simp
-next case (Unfold e)
-  thus ?case by simp
-next case (TyLam e) 
-  thus ?case by simp
-next case (TyAp t e)
-  thus ?case by simp
-qed 
-
-lemma [simp]: "sub_from n (subst' (incr_from n e) e' n) = e" 
-by (induction e arbitrary: n e', simp_all add: incr_def)
-
-lemma [simp]: "subst (incr_from 0 e) e' = e"
-by (simp add: subst_def) 
-
-primrec subst_type' :: "expr => type => nat => expr"
-where "subst_type' (Var v) e x = Var v"
-    | "subst_type' (Lam t b) e x = Lam (type_subst' t e x) (subst_type' b e x)"
-    | "subst_type' (Ap e1 e2) e x = Ap (subst_type' e1 e x) (subst_type' e2 e x)"
-    | "subst_type' (Fix t b) e x = Fix (type_subst' t e x) (subst_type' b e x)"
-    | "subst_type' Triv e x = Triv"
-    | "subst_type' (Pair e1 e2) e x = Pair (subst_type' e1 e x) (subst_type' e2 e x)"
-    | "subst_type' (ProjL n) e x = ProjL (subst_type' n e x)"
-    | "subst_type' (ProjR n) e x = ProjR (subst_type' n e x)"
-    | "subst_type' (Abort t n) e x = Abort (type_subst' t e x) (subst_type' n e x)"
-    | "subst_type' (InL t t' n) e x = InL (type_subst' t e x) (type_subst' t' e x) (subst_type' n e x)"
-    | "subst_type' (InR t t' n) e x = InR (type_subst' t e x) (type_subst' t' e x) (subst_type' n e x)"
-    | "subst_type' (Case n el er) e x = Case (subst_type' n e x) (subst_type' el e x) (subst_type' er e x)"
-    | "subst_type' (Fold t n) e x = Fold (type_subst' t e x) (subst_type' n e x)"
-    | "subst_type' (Unfold n) e x = Unfold (subst_type' n e x)"
-    | "subst_type' (TyLam n) e x = TyLam (subst_type' n e (Suc x))"
-    | "subst_type' (TyAp t n) e x = TyAp (type_subst' t e x) (subst_type' n e x)"
-
-primrec sub_type_from :: "expr => nat => expr"
-where "sub_type_from (Var v) n = Var v"
-    | "sub_type_from (Lam t b) n = Lam (type_sub_from n t) (sub_type_from b n)"
-    | "sub_type_from (Ap e1 e2) n = Ap (sub_type_from e1 n) (sub_type_from e2 n)"
-    | "sub_type_from (Fix t b) n = Fix (type_sub_from n t) (sub_type_from b n)"
-    | "sub_type_from Triv n = Triv"
-    | "sub_type_from (Pair e1 e2) n = Pair (sub_type_from e1 n) (sub_type_from e2 n)"
-    | "sub_type_from (ProjL e) n = ProjL (sub_type_from e n)"
-    | "sub_type_from (ProjR e) n = ProjR (sub_type_from e n)"
-    | "sub_type_from (Abort t e) n = Abort (type_sub_from n t) (sub_type_from e n)"
-    | "sub_type_from (InL t t' e) n = InL (type_sub_from n t) (type_sub_from n t') (sub_type_from e n)"
-    | "sub_type_from (InR t t' e) n = InR (type_sub_from n t) (type_sub_from n t') (sub_type_from e n)"
-    | "sub_type_from (Case e el er) n = Case (sub_type_from e n) (sub_type_from el n) (sub_type_from er n)"
-    | "sub_type_from (Fold t e) n = Fold (type_sub_from n t) (sub_type_from e n)"
-    | "sub_type_from (Unfold e) n = Unfold (sub_type_from e n)"
-    | "sub_type_from (TyLam e) n = TyLam (sub_type_from e (Suc n))"
-    | "sub_type_from (TyAp t e) n = TyAp (type_sub_from n t) (sub_type_from e n)"
-
-definition subst_type :: "expr => type => expr"
-where "subst_type e t = sub_type_from (subst_type' e (type_incr_from 0 t) 0) 0"
+lemma [simp]: "canswap m n ==> insert m (insert n e) = insert (next n) (insert m e)"
+by (induction e arbitrary: n m, simp_all)
 
 end
