isabelle/Chapter20_2_Typechecking.thy
@@ -2,277 +2,53 @@ theory Chapter20_2_Typechecking
 imports Chapter20_1_Language
 begin
 
-primrec verify_types :: "nat set => expr => bool"
-where "verify_types tvs (Var v) = True"
-    | "verify_types tvs (Lam t b) = (is_valid_type tvs t & verify_types tvs b)"
-    | "verify_types tvs (Ap e1 e2) = (verify_types tvs e1 & verify_types tvs e2)"
-    | "verify_types tvs (Fix t b) = (is_valid_type tvs t & verify_types tvs b)"
-    | "verify_types tvs Triv = True"
-    | "verify_types tvs (Pair e1 e2) = (verify_types tvs e1 & verify_types tvs e2)"
-    | "verify_types tvs (ProjL n) = verify_types tvs n"
-    | "verify_types tvs (ProjR n) = verify_types tvs n"
-    | "verify_types tvs (Abort t n) = (is_valid_type tvs t & verify_types tvs n)"
-    | "verify_types tvs (InL t t' n) = (is_valid_type tvs t & is_valid_type tvs t' & verify_types tvs n)"
-    | "verify_types tvs (InR t t' n) = (is_valid_type tvs t & is_valid_type tvs t' & verify_types tvs n)"
-    | "verify_types tvs (Case n el er) = (verify_types tvs n & verify_types tvs el & verify_types tvs er)"
-    | "verify_types tvs (Fold t n) = (is_valid_type tvs t & verify_types tvs n)"
-    | "verify_types tvs (Unfold n) = verify_types tvs n"
-    | "verify_types tvs (TyLam n) = verify_types (expand_set tvs) n"
-    | "verify_types tvs (TyAp t n) = (is_valid_type tvs t & verify_types tvs n)"
+inductive typecheck :: "type env => expr => type => bool"
+where tc_var [simp]: "lookup gam x = Some t ==> typecheck gam (Var x) t"
+    | tc_zero [simp]: "typecheck gam Zero Nat"
+    | tc_suc [simp]: "typecheck gam e Nat ==> typecheck gam (Suc e) Nat"
+    | tc_rec [simp]: "typecheck gam et Nat ==> typecheck gam e0 t ==> 
+                typecheck (extend (extend gam t) Nat) es t ==> typecheck gam (Rec et e0 es) t"
+    | tc_lam [simp]: "typecheck (extend gam t1) e t2 ==> typecheck gam (Lam t1 e) (Arrow t1 t2)"
+    | tc_appl [simp]: "typecheck gam e1 (Arrow t2 t) ==> typecheck gam e2 t2 ==> 
+                typecheck gam (Appl e1 e2) t"
+    | tc_triv [simp]: "typecheck gam Triv Unit"
+    | tc_pair [simp]: "typecheck gam e1 t1 ==> typecheck gam e2 t2 ==> 
+                typecheck gam (Pair e1 e2) (Prod t1 t2)"
+    | tc_projl [simp]: "typecheck gam e (Prod t1 t2) ==> typecheck gam (ProjL e) t1"
+    | tc_projr [simp]: "typecheck gam e (Prod t1 t2) ==> typecheck gam (ProjR e) t2"
+    | tc_abort [simp]: "typecheck gam e Void ==> typecheck gam (Abort t e) t"
+    | tc_case [simp]: "typecheck gam et (Sum t1 t2) ==> typecheck (extend gam t1) el t ==> 
+                typecheck (extend gam t2) er t ==> typecheck gam (Case et el er) t"
+    | tc_inl [simp]: "typecheck gam e t1 ==> typecheck gam (InL t1 t2 e) (Sum t1 t2)"
+    | tc_inr [simp]: "typecheck gam e t2 ==> typecheck gam (InR t1 t2 e) (Sum t1 t2)"
 
-inductive typecheck :: "(nat, type) assoc => expr => type => bool"
-where tvar [simp]: "lookup env v = Some t ==> typecheck env (Var v) t"
-    | tlam [simp]: "typecheck (extend_at env 0 r) e t ==> typecheck env (Lam r e) (Arr r t)"
-    | tapp [simp]: "typecheck env e1 (Arr t2 t) ==> typecheck env e2 t2 ==> 
-                        typecheck env (Ap e1 e2) t"
-    | tfix [simp]: "typecheck (extend_at env 0 t) b t ==> typecheck env (Fix t b) t"
-    | ttrv [simp]: "typecheck env Triv Unit"
-    | tpar [simp]: "typecheck env e1 t1 ==> typecheck env e2 t2 ==> typecheck env (Pair e1 e2) (Prod t1 t2)"
-    | tprl [simp]: "typecheck env e (Prod t1 t2) ==> typecheck env (ProjL e) t1"
-    | tprr [simp]: "typecheck env e (Prod t1 t2) ==> typecheck env (ProjR e) t2"
-    | tabt [simp]: "typecheck env e Void ==> typecheck env (Abort t e) t"
-    | tinl [simp]: "typecheck env e t1 ==> typecheck env (InL t1 t2 e) (Sum t1 t2)"
-    | tinr [simp]: "typecheck env e t2 ==> typecheck env (InR t1 t2 e) (Sum t1 t2)"
-    | tcse [simp]: "typecheck env e (Sum t1 t2) ==> typecheck (extend_at env 0 t1) el t ==> 
-                        typecheck (extend_at env 0 t2) er t ==> typecheck env (Case e el er) t"
-    | tfld [simp]: "typecheck env e (type_subst t (Rec t)) ==> typecheck env (Fold t e) (Rec t)"
-    | tufd [simp]: "typecheck env e (Rec t) ==> typecheck env (Unfold e) (type_subst t (Rec t))"
-    | ttlm [simp]: "typecheck env e t ==> typecheck env (TyLam e) (All t)"
-    | ttap [simp]: "typecheck env e (All t1) ==> typecheck env (TyAp t e) (type_subst t1 t)"
+inductive_cases [elim!]: "typecheck gam (Var x) t"
+inductive_cases [elim!]: "typecheck gam Zero t"
+inductive_cases [elim!]: "typecheck gam (Suc e) t"
+inductive_cases [elim!]: "typecheck gam (Rec et e0 es) t"
+inductive_cases [elim!]: "typecheck gam (Lam t1 e) t"
+inductive_cases [elim!]: "typecheck gam (Appl e1 e2) t"
+inductive_cases [elim!]: "typecheck gam (TyLam e) t"
+inductive_cases [elim!]: "typecheck gam (TyAppl e1 e2) t"
+inductive_cases [elim!]: "typecheck gam Triv t"
+inductive_cases [elim!]: "typecheck gam (Pair e1 e2) t"
+inductive_cases [elim!]: "typecheck gam (ProjL e) t"
+inductive_cases [elim!]: "typecheck gam (ProjR e) t"
+inductive_cases [elim!]: "typecheck gam (Abort t1 e) t"
+inductive_cases [elim!]: "typecheck gam (Case et el er) t"
+inductive_cases [elim!]: "typecheck gam (InL t1 t2 e) t"
+inductive_cases [elim!]: "typecheck gam (InR t1 t2 e) t"
 
-inductive_cases [elim!]: "typecheck e (Var x) t"
-inductive_cases [elim!]: "typecheck e (Lam x y) t"
-inductive_cases [elim!]: "typecheck e (Ap x y) t"
-inductive_cases [elim!]: "typecheck e (Fix x y) t"
-inductive_cases [elim!]: "typecheck e Triv t"
-inductive_cases [elim!]: "typecheck e (Pair x y) t"
-inductive_cases [elim!]: "typecheck e (ProjL x) t"
-inductive_cases [elim!]: "typecheck e (ProjR x) t"
-inductive_cases [elim!]: "typecheck e (Abort x y) t"
-inductive_cases [elim!]: "typecheck e (InL x y z) t"
-inductive_cases [elim!]: "typecheck e (InR x y z) t"
-inductive_cases [elim!]: "typecheck e (Case x y z) t"
-inductive_cases [elim!]: "typecheck e (Fold x y) t"
-inductive_cases [elim!]: "typecheck e (Unfold x) t"
-inductive_cases [elim!]: "typecheck e (TyLam x) t"
-inductive_cases [elim!]: "typecheck e (TyAp x y) t"
+lemma [simp]: "typecheck gam e t ==> n in gam ==> 
+         typecheck (extend_at n gam t') (insert n e) t"
+by (induction gam e t arbitrary: n rule: typecheck.induct, fastforce+)
 
-lemma [simp]: "typecheck env e t ==> typecheck (extend_at env n k) (incr_from n e) t"
-proof (induction env e t arbitrary: n rule: typecheck.inducts)
-case tvar
-  thus ?case by (simp add: incr_def)
-next case (tlam env r b t)
-  hence "typecheck (extend_at (extend_at env 0 r) (Suc n) k) (incr_from (Suc n) b) t" by simp
-  thus ?case by (simp add: extend_at_swap)
-next case (tapp env e1 t2 t e2)
-  from tapp have "typecheck (extend_at env n k) (incr_from n e1) (Arr t2 t)" by simp
-  moreover from tapp have "typecheck (extend_at env n k) (incr_from n e2) t2" by simp
-  ultimately show ?case by simp
-next case (tfix env t b)
-  hence "typecheck (extend_at (extend_at env 0 t) (Suc n) k) (incr_from (Suc n) b) t" by simp
-  thus ?case by (simp add: extend_at_swap)
-next case ttrv
-  thus ?case by simp
-next case tpar
-  thus ?case by simp
-next case (tprl env e t1 t2)
-  hence "typecheck (extend_at env n k) (incr_from n e) (Prod t1 t2)" by simp
-  thus ?case by simp 
-next case (tprr env e t1 t2)
-  hence "typecheck (extend_at env n k) (incr_from n e) (Prod t1 t2)" by simp
-  thus ?case by simp
-next case tabt
-  thus ?case by simp
-next case tinl
-  thus ?case by simp
-next case tinr
-  thus ?case by simp
-next case (tcse env e t1 t2 el t er)
-  hence "typecheck (extend_at env n k) (incr_from n e) (Sum t1 t2)" by simp 
-  moreover from tcse have "typecheck (extend_at (extend_at env 0 t1) (Suc n) k) (incr_from (Suc n) el) t" by simp
-  moreover from tcse have "typecheck (extend_at (extend_at env 0 t2) (Suc n) k) (incr_from (Suc n) er) t" by simp
-  ultimately show ?case by (simp add: extend_at_swap)
-next case tfld
-  thus ?case by simp
-next case tufd
-  thus ?case by simp
-next case ttlm
-  thus ?case by simp
-next case ttap
-  thus ?case by simp
-qed
+lemma [simp]: "typecheck (extend_at n gam t') e t ==> n in gam ==> typecheck gam e' t' ==> 
+        typecheck gam (remove n (subst' n (insert n e') e)) t"
+by (induction "extend_at n gam t'" e t arbitrary: n gam t' e' rule: typecheck.induct, fastforce+)
 
-lemma [simp]: "typecheck env e t ==> typecheck (extend_env ts env) (incr_by (length ts) e) t"
-by (induction ts, simp_all)        
-
-lemma [simp]: "typecheck (extend_at env n k) e t ==> n ~: free_vars e ==> typecheck env (sub_from n e) t"
-proof (induction "extend_at env n k" e t arbitrary: env n rule: typecheck.inducts)
-case (tvar v t)
-  thus ?case by (cases "v < n", simp, cases "v = n", simp_all)
-next case tlam
-  thus ?case by (simp add: extend_at_swap)
-next case (tapp e1 t2 t e2)
-  from tapp have "typecheck env (sub_from n e1) (Arr t2 t)" by simp
-  moreover from tapp have "typecheck env (sub_from n e2) t2" by simp
-  ultimately show ?case by simp
-next case tfix
-  thus ?case by (simp add: extend_at_swap)
-next case ttrv
-  thus ?case by simp
-next case tpar
-  thus ?case by simp
-next case (tprl e t1 t2)
-  hence "typecheck env (sub_from n e) (Prod t1 t2)" by simp
-  thus ?case by simp
-next case (tprr e t1 t2)
-  hence "typecheck env (sub_from n e) (Prod t1 t2)" by simp
-  thus ?case by simp
-next case tabt
-  thus ?case by simp
-next case tinl
-  thus ?case by simp
-next case tinr
-  thus ?case by simp
-next case (tcse e t1 t2 el t er)
-  hence "typecheck env (sub_from n e) (Sum t1 t2)" by simp 
-  moreover from tcse have "typecheck (extend_at env 0 t1) (sub_from (Suc n) el) t" by (simp add: extend_at_swap)
-  moreover from tcse have "typecheck (extend_at env 0 t2) (sub_from (Suc n) er) t" by (simp add: extend_at_swap)
-  ultimately show ?case by simp
-next case tfld
-  thus ?case by simp
-next case tufd
-  thus ?case by simp
-next case ttlm
-  thus ?case by simp
-next case ttap
-  thus ?case by simp
-qed
-
-lemma [simp]: "typecheck (extend env x t2) e t1 ==> typecheck env eb t2 ==> typecheck env (subst' e eb x) t1"
-proof (induction "extend env x t2" e t1 arbitrary: env eb x rule: typecheck.inducts)
-case tvar
-  thus ?case by auto
-next case tlam
-  thus ?case by simp
-next case (tapp e1 t2 t e2)
-  from tapp have "typecheck env (subst' e1 eb x) (Arr t2 t)" by simp
-  moreover from tapp have "typecheck env (subst' e2 eb x) t2" by simp
-  ultimately show ?case by simp
-next case tfix
-  thus ?case by simp
-next case ttrv
-  thus ?case by simp
-next case tpar
-  thus ?case by simp
-next case (tprl e t1 t2)
-  hence "typecheck env (subst' e eb x) (Prod t1 t2)" by simp
-  thus ?case by simp
-next case (tprr e t1 t2)
-  hence "typecheck env (subst' e eb x) (Prod t1 t2)" by simp
-  thus ?case by simp
-next case tabt
-  thus ?case by simp
-next case tinl
-  thus ?case by simp
-next case tinr
-  thus ?case by simp
-next case (tcse e t1 t2 el t er)
-  hence "typecheck env (subst' e eb x) (Sum t1 t2)" by (simp add: extend_at_swap) 
-  moreover from tcse have "typecheck (extend_at env 0 t1) (subst' el (incr_from 0 eb) (Suc x)) t" by (simp add: extend_at_swap) 
-  moreover from tcse have "typecheck (extend_at env 0 t2) (subst' er (incr_from 0 eb) (Suc x)) t" by (simp add: extend_at_swap) 
-  ultimately show ?case by simp
-next case tfld
-  thus ?case by simp
-next case tufd
-  thus ?case by simp
-next case ttlm
-  thus ?case by simp
-next case ttap
-  thus ?case by simp
-qed
-
-lemma [simp]: "typecheck (extend_at env 0 t') e t ==> typecheck env e' t' ==> typecheck env (subst e e') t"
+lemma [simp]: "typecheck (extend gam t') e t ==> typecheck gam e' t' ==> 
+                          typecheck gam (subst e' e) t"
 by (simp add: subst_def)
-
-lemma [simp]: "is_valid_type (expand_set_at n tvs) t ==> is_valid_type tvs t' ==> 
-      is_valid_type tvs (type_sub_from n (type_subst' t (type_incr_from n t') n))"
-by (induction t arbitrary: tvs t' n, auto) 
-
-lemma [simp]: "is_valid_type (expand_set tvs) t ==> is_valid_type tvs t' ==> is_valid_type tvs (type_subst t t')"
-by (simp add: type_subst_def)
-
-lemma [simp]: "typecheck env e t ==> 
-            typecheck (assoc_map (%t. type_sub_from n (type_subst' t (type_incr_from n t') n)) env) 
-                      (sub_type_from (subst_type' e (type_incr_from n t') n) n) 
-                      (type_sub_from n (type_subst' t (type_incr_from n t') n))"
-proof (induction env e t arbitrary: n t' rule: typecheck.inducts)
-case tvar
-  thus ?case by simp
-next case tlam
-  thus ?case by simp
-next case (tapp env e1 t2 t e2)
-  hence X: "typecheck (assoc_map (\<lambda>t. type_sub_from n (type_subst' t (type_incr_from n t') n)) env) 
-                  (sub_type_from (subst_type' e1 (type_incr_from n t') n) n) 
-                  (Arr (type_sub_from n (type_subst' t2 (type_incr_from n t') n)) 
-                       (type_sub_from n (type_subst' t (type_incr_from n t') n)))" by simp
-  from tapp have "typecheck (assoc_map (\<lambda>t. type_sub_from n (type_subst' t (type_incr_from n t') n)) env) 
-              (sub_type_from (subst_type' e2  (type_incr_from n t') n) n) 
-              (type_sub_from n (type_subst' t2 (type_incr_from n t') n))" by simp                 
-  with X show ?case by simp
-next case tfix
-  thus ?case by simp
-next case ttrv
-  thus ?case by simp
-next case tpar
-  thus ?case by simp
-next case tprl
-  thus ?case by (metis sub_type_from.simps(7) subst_type'.simps(7) type_sub_from.simps(4) type_subst'.simps(4) typecheck.tprl)
-next case tprr
-  thus ?case by (metis sub_type_from.simps(8) subst_type'.simps(8) type_sub_from.simps(4) type_subst'.simps(4) typecheck.tprr)
-next case tabt
-  thus ?case by simp
-next case tinl
-  thus ?case by simp
-next case tinr
-  thus ?case by simp
-next case (tcse env e t1 t2 el t er)
-  from tcse have X: "typecheck 
-   (assoc_map (\<lambda>t. type_sub_from n (type_subst' t (type_incr_from n t') n)) env) 
-   (sub_type_from (subst_type' e (type_incr_from n t') n) n) 
-   (Sum (type_sub_from n (type_subst' t1 (type_incr_from n t') n)) (type_sub_from n (type_subst' t2 (type_incr_from n t') n)))" by simp
-  from tcse have Y: "typecheck 
-    (extend_at (assoc_map (\<lambda>t. type_sub_from n (type_subst' t (type_incr_from n t') n)) env) 0 (type_sub_from n (type_subst' t1 (type_incr_from n t') n))) 
-    (sub_type_from (subst_type' el (type_incr_from n t') n) n) 
-    (type_sub_from n (type_subst' t (type_incr_from n t') n))" by simp
-  from tcse have Z: "typecheck 
-    (extend_at (assoc_map (\<lambda>t. type_sub_from n (type_subst' t (type_incr_from n t') n)) env) 0 (type_sub_from n (type_subst' t2 (type_incr_from n t') n))) 
-    (sub_type_from (subst_type' er (type_incr_from n t') n) n) 
-    (type_sub_from n (type_subst' t (type_incr_from n t') n))" by simp
-  from X Y Z show ?case by simp
-next case (tfld env e t)
-  from tfld have "typecheck env e (type_subst t (Rec t))" by simp
-  from tfld have "typecheck 
-    (assoc_map (\<lambda>t. type_sub_from nn (type_subst' t (type_incr_from nn tt') nn)) env)
-   (sub_type_from (subst_type' e (type_incr_from nn tt') nn) nn)
-   (type_sub_from nn (type_subst' (type_subst t (Rec t)) (type_incr_from nn tt') nn))" by simp
-
-
-  have "typecheck eenv ee (type_subst tt (Rec tt)) ==> typecheck eenv (Fold tt ee) (Rec tt)" by simp
-
-  hence "typecheck 
-          (assoc_map (\<lambda>t. type_sub_from n (type_subst' t (type_incr_from n t') n)) env)
-          (Fold (type_sub_from n (type_subst' t (type_incr_from n t') n)) (sub_type_from (subst_type' e (type_incr_from n t') n) n))
-           (Rec (type_sub_from (Suc n) (type_subst' t (type_incr_from (Suc n) (type_incr_from 0 t')) (Suc n))))" by simp sorry
-  thus ?case by simp
-next case tufd
-  thus ?case by simp sorry
-next case ttlm
-  thus ?case by simp sorry
-next case ttap
-  thus ?case by simp sorry
-qed
-
-lemma [simp]: "typecheck env e t ==> typecheck (assoc_map (%t. type_subst t t') env) (subst_type e t') (type_subst t t')"
-by (simp add: subst_type_def type_subst_def)
 
 end
