isabelle/Chapter20_3_Evaluation.thy
@@ -2,342 +2,146 @@ theory Chapter20_3_Evaluation
 imports Chapter20_2_Typechecking
 begin
 
-fun is_val :: "expr => bool"
+primrec is_val :: "expr => bool"
 where "is_val (Var v) = False"
-    | "is_val (Lam t b) = True"
-    | "is_val (Ap e1 e2) = False"
-    | "is_val (Fix t b) = False"
+    | "is_val Zero = True"
+    | "is_val (Suc e) = is_val e"
+    | "is_val (Rec et e0 es) = False"
+    | "is_val (Lam t e) = True"
+    | "is_val (Appl e1 e2) = False"
+    | "is_val (TyLam e) = True"
+    | "is_val (TyAppl t e) = False"
     | "is_val Triv = True"
     | "is_val (Pair e1 e2) = (is_val e1 & is_val e2)"
     | "is_val (ProjL e) = False"
     | "is_val (ProjR e) = False"
     | "is_val (Abort t e) = False"
-    | "is_val (InL t t' e) = is_val e"
-    | "is_val (InR t t' e) = is_val e"
-    | "is_val (Case e el er) = False"
-    | "is_val (Fold t e) = is_val e"
-    | "is_val (Unfold e) = False"
-    | "is_val (TyLam b) = True"
-    | "is_val (TyAp e1 e2) = False"
-
-lemma canonical_arr: "typecheck env e (Arr t1 t2) ==> is_val e ==> (EX v. e = Lam t1 v & typecheck (extend_at env 0 t1) v t2)"
-by (induction e, auto)
-
-lemma canonical_unit: "typecheck env e Unit ==> is_val e ==> e = Triv"
-by (induction e, auto)
-
-lemma canonical_prod: "typecheck env e (Prod t1 t2) ==> is_val e ==> (EX e1 e2. e = Pair e1 e2 & typecheck env e1 t1 & typecheck env e2 t2 & is_val e1 & is_val e2)"
-by (induction e, auto)
-
-lemma canonical_void: "typecheck env e Void ==> ~ is_val e"
-by (induction e, auto)
-
-lemma canonical_sum: "typecheck env e (Sum t1 t2) ==> is_val e ==> 
-      (EX e'. e = InL t1 t2 e' & is_val e' & typecheck env e' t1) | (EX e'. e = InR t1 t2 e' & is_val e' & typecheck env e' t2)"
-by (induction e, auto)
-
-lemma canonical_rec: "typecheck env e (Rec t) ==> is_val e ==> EX e'. e = Fold t e' & is_val e'"
-by (induction e, auto)
-
-lemma canonical_all: "typecheck env e (All t) ==> is_val e ==> (EX v. e = TyLam v & typecheck env v t)"
-by (induction e, auto)
+    | "is_val (Case et el er) = False"
+    | "is_val (InL t1 t2 e) = is_val e"
+    | "is_val (InR t1 t2 e) = is_val e"
 
 inductive eval :: "expr => expr => bool"
-where eap1 [simp]: "eval e1 e1' ==> eval (Ap e1 e2) (Ap e1' e2)"
-    | eap2 [simp]: "is_val e1 ==> eval e2 e2' ==> eval (Ap e1 e2) (Ap e1 e2')"
-    | eap3 [simp]: "is_val e2 ==> eval (Ap (Lam t b) e2) (subst b e2)"
-    | efix [simp]: "eval (Fix t b) (subst b (Fix t b))"
-    | epa1 [simp]: "eval e1 e1' ==> eval (Pair e1 e2) (Pair e1' e2)"
-    | epa2 [simp]: "is_val e1 ==> eval e2 e2' ==> eval (Pair e1 e2) (Pair e1 e2')"
-    | epl1 [simp]: "eval e e' ==> eval (ProjL e) (ProjL e')"
-    | epl2 [simp]: "is_val e1 ==> is_val e2 ==> eval (ProjL (Pair e1 e2)) e1"
-    | epr1 [simp]: "eval e e' ==> eval (ProjR e) (ProjR e')"
-    | epr2 [simp]: "is_val e1 ==> is_val e2 ==> eval (ProjR (Pair e1 e2)) e2"
-    | eabt [simp]: "eval e e' ==> eval (Abort t e) (Abort t e')"
-    | einl [simp]: "eval e e' ==> eval (InL t t' e) (InL t t' e')"
-    | einr [simp]: "eval e e' ==> eval (InR t t' e) (InR t t' e')"
-    | ecs1 [simp]: "eval e e' ==> eval (Case e el er) (Case e' el er)"
-    | ecs2 [simp]: "is_val e ==> eval (Case (InL t t' e) el er) (subst el e)"
-    | ecs3 [simp]: "is_val e ==> eval (Case (InR t t' e) el er) (subst er e)"
-    | efld [simp]: "eval e e' ==> eval (Fold t e) (Fold t e')"
-    | euf1 [simp]: "eval e e' ==> eval (Unfold e) (Unfold e')"
-    | euf2 [simp]: "is_val e ==> eval (Unfold (Fold t e)) e"
-    | eta1 [simp]: "eval (TyAp t (TyLam e)) (subst_type e t)"
-    | eta2 [simp]: "eval e e' ==> eval (TyAp t e) (TyAp t e')"
+where eval_suc [simp]: "eval e e' ==> eval (Suc e) (Suc e')"
+    | eval_rec_1 [simp]: "eval et et' ==> eval (Rec et e0 es) (Rec et' e0 es)"
+    | eval_rec_2 [simp]: "eval (Rec Zero e0 es) e0"
+    | eval_rec_3 [simp]: "is_val et ==> 
+            eval (Rec (Suc et) e0 es) (subst (Rec et e0 es) (subst et es))"
+    | eval_appl_1 [simp]: "eval e1 e1' ==> eval (Appl e1 e2) (Appl e1' e2)"
+    | eval_appl_2 [simp]: "is_val e1 ==> eval e2 e2' ==> eval (Appl e1 e2) (Appl e1 e2')"
+    | eval_appl_3 [simp]: "is_val e2 ==> eval (Appl (Lam t2 e1) e2) (subst e2 e1)"
+    | eval_pair_1 [simp]: "eval e1 e1' ==> eval (Pair e1 e2) (Pair e1' e2)"
+    | eval_pair_2 [simp]: "is_val e1 ==> eval e2 e2' ==> eval (Pair e1 e2) (Pair e1 e2')"
+    | eval_projl_1 [simp]: "eval e e' ==> eval (ProjL e) (ProjL e')"
+    | eval_projl_2 [simp]: "eval (ProjL (Pair e1 e2)) e1"
+    | eval_projr_1 [simp]: "eval e e' ==> eval (ProjR e) (ProjR e')"
+    | eval_projr_2 [simp]: "eval (ProjR (Pair e1 e2)) e2"
+    | eval_abort [simp]: "eval e e' ==> eval (Abort t e) (Abort t e')"
+    | eval_case_1 [simp]: "eval et et' ==> eval (Case et el er) (Case et' el er)"
+    | eval_case_2 [simp]: "is_val e ==> eval (Case (InL t1 t2 e) el er) (subst e el)"
+    | eval_case_3 [simp]: "is_val e ==> eval (Case (InR t1 t2 e) el er) (subst e er)"
+    | eval_inl [simp]: "eval e e' ==> eval (InL t1 t2 e) (InL t1 t2 e')"
+    | eval_inr [simp]: "eval e e' ==> eval (InR t1 t2 e) (InR t1 t2 e')"
 
-theorem preservation: "eval e e' ==> env = empty_map ==> typecheck env e t ==> typecheck env e' t"
-proof (induction e e' arbitrary: t env rule: eval.inducts)
-next case (eap1 e1 e1' e2)
-  hence "EX t2. typecheck env e1' (Arr t2 t) & typecheck env e2 t2" by auto
-  thus ?case by auto
-next case (eap2 e1 e2 e2')
-  thus ?case by auto
-next case eap3
-  thus ?case by auto
-next case efix
-  thus ?case by auto
-next case epa1
-  thus ?case by auto
-next case epa2
-  thus ?case by auto
-next case (epl1 e e')
-  hence "!!t2. typecheck env e (Prod t t2) ==> typecheck env e' (Prod t t2)" by simp
-  with epl1 have "EX t2. typecheck env e' (Prod t t2)" by auto
-  thus ?case by auto
-next case epl2
-  thus ?case by auto
-next case (epr1 e e')
-  hence "!!t1. typecheck env e (Prod t1 t) ==> typecheck env e' (Prod t1 t)" by simp
-  with epr1 have "EX t1. typecheck env e' (Prod t1 t)" by auto
-  thus ?case by auto
-next case epr2
-  thus ?case by auto
-next case eabt
-  thus ?case by auto
-next case einl
-  thus ?case by auto
-next case einr
-  thus ?case by auto
-next case (ecs1 e e' el er)
-  then obtain t1 t2 where T: "typecheck env e (Sum t1 t2) & 
-                            typecheck (extend_at env 0 t1) el t & 
-                            typecheck (extend_at env 0 t2) er t" by auto
-  with ecs1 have "typecheck env e' (Sum t1 t2)" by simp
-  with T show ?case by simp
-next case ecs2
-  thus ?case by auto
-next case ecs3
-  thus ?case by auto
-next case efld
-  thus ?case by auto
-next case euf1
-  thus ?case by auto
-next case euf2
-  thus ?case by auto
-next case (eta1 t' e)
-  then obtain t1 where T: "typecheck empty_map e t1 & t = type_subst t1 t'" by auto
-  hence T2: "typecheck empty_map e t1" by simp
-  have "!!env. typecheck env e t1 ==> typecheck (assoc_map (%t. type_subst t t') env) (subst_type e t') (type_subst t1 t')" by simp
-  with T2 have "typecheck (assoc_map (%t. type_subst t t') empty_map) (subst_type e t') (type_subst t1 t')" by fast
-  with T eta1 show ?case by simp
-next case eta2
-  thus ?case by auto
+lemma canonical_nat: "is_val e ==> typecheck gam e Nat ==> 
+          e = Zero | (EX e'. e = Suc e' & typecheck gam e' Nat)"
+by (induction e, auto)
+
+lemma canonical_nat_no_vars: "is_val e ==> typecheck gam e Nat ==> typecheck gam' e Nat"
+by (induction e, auto) 
+
+lemma canonical_arrow: "is_val e ==> typecheck gam e (Arrow t1 t2) ==> 
+              EX e'. e = Lam t1 e' & typecheck (extend gam t1) e' t2"
+by (induction e, auto)
+
+lemma canonical_unit: "is_val e ==> typecheck gam e Unit ==> e = Triv"
+by (induction e, auto)
+
+lemma canonical_prod: "is_val e ==> typecheck gam e (Prod t1 t2) ==> 
+              EX e1 e2. e = Pair e1 e2 & typecheck gam e1 t1 & typecheck gam e2 t2"
+by (induction e, auto)
+
+lemma canonical_void: "is_val e ==> typecheck gam e Void ==> False"
+by (induction e, auto)
+
+lemma canonical_sum: "is_val e ==> typecheck gam e (Sum t1 t2) ==> 
+          (EX e'. e = InL t1 t2 e' & typecheck gam e' t1) | 
+          (EX e'. e = InR t1 t2 e' & typecheck gam e' t2)"
+by (induction e, auto)
+
+theorem preservation: "eval e e' ==> typecheck gam e t ==> typecheck gam e' t"
+proof (induction e e' arbitrary: t rule: eval.induct)
+case eval_suc 
+  thus ?case by fastforce
+next case eval_rec_1 
+  thus ?case by fastforce
+next case eval_rec_2 
+  thus ?case by fastforce
+next case (eval_rec_3 et e0 es)
+  from eval_rec_3 canonical_nat_no_vars have "typecheck (extend gam t) (subst et es) t" by auto
+  with eval_rec_3 show ?case by fastforce
+next case eval_appl_1 
+  thus ?case by fastforce
+next case eval_appl_2 
+  thus ?case by fastforce
+next case eval_appl_3 
+  thus ?case by fastforce
+next case eval_pair_1 
+  thus ?case by fastforce
+next case eval_pair_2 
+  thus ?case by fastforce
+next case eval_projl_1 
+  thus ?case by fastforce
+next case eval_projl_2 
+  thus ?case by fastforce
+next case eval_projr_1 
+  thus ?case by fastforce
+next case eval_projr_2 
+  thus ?case by fastforce
+next case eval_abort
+  thus ?case by fastforce
+next case eval_case_1 
+  thus ?case by fastforce
+next case eval_case_2 
+  thus ?case by fastforce
+next case eval_case_3 
+  thus ?case by fastforce
+next case eval_inl
+  thus ?case by fastforce
+next case eval_inr
+  thus ?case by fastforce
 qed
 
-theorem progress: "typecheck env e t ==> env = empty_map ==> is_val e | (EX e'. eval e e')"
-proof (induction env e t arbitrary: rule: typecheck.inducts)
-case tvar
-  thus ?case by auto
-next case tlam
+theorem progress: "typecheck gam e t ==> gam = empty_env ==> is_val e | (EX e'. eval e e')"
+proof (induction gam e t rule: typecheck.induct)
+case tc_var
   thus ?case by simp
-next case (tapp env e1 t2 t e2)
-  show ?case
-  proof (cases "is_val e1")
-  case True
-    with tapp have "EX v. e1 = Lam t2 v & typecheck (extend_at env 0 t2) v t" by (simp add: canonical_arr)
-    hence e1_is_lam: "EX v. e1 = Lam t2 v" by auto
-    thus ?thesis 
-    proof (cases "is_val e2")
-    case True
-      with e1_is_lam show ?thesis
-      proof auto
-        fix v
-        assume "is_val e2"
-        hence "eval (Ap (Lam t2 v) e2) (subst v e2)" by simp
-        thus "EX x. eval (Ap (Lam t2 v) e2) x" by auto
-      qed
-    next case False
-      with tapp have "\<exists>a. eval e2 a" by auto
-      thus ?thesis
-      proof auto
-        fix a
-        assume "eval e2 a"
-        moreover from True have "is_val e1" by simp
-        ultimately have "eval (Ap e1 e2) (Ap e1 a)" by simp
-        thus "EX x. eval (Ap e1 e2) x" by auto
-      qed
-    qed
-  next case False
-    with tapp have "\<exists>a. eval e1 a" by auto
-    thus ?thesis
-    proof auto
-      fix a
-      assume "eval e1 a"
-      hence "eval (Ap e1 e2) (Ap a e2)" by simp
-      thus "EX x. eval (Ap e1 e2) x" by auto
-    qed
-  qed
-next case (tfix env t b)
-  def b' == "subst b (Fix t b)"
-  have "eval (Fix t b) b'" by (simp add: b'_def)
-  thus ?case by auto
-next case ttrv
+next case tc_zero
   thus ?case by simp
-next case (tpar env e1 t1 e2 t2)
-  thus ?case
-  proof (cases "is_val e1")
-  case True
-    hence X: "is_val e1" by simp
-    thus ?thesis
-    proof (cases "is_val e2")
-    case True
-      with X show ?thesis by simp  
-    next case False
-      with tpar have "EX a. eval e2 a" by auto
-      hence "EX a. eval (Pair e1 e2) a"
-      proof auto
-        fix e2'
-        assume "eval e2 e2'"
-        with True have "eval (Pair e1 e2) (Pair e1 e2')" by simp
-        thus "EX a. eval (Pair e1 e2) a" by auto
-      qed
-      thus ?thesis by simp  
-    qed
-  next case False
-    with tpar have "EX a. eval e1 a" by auto
-    hence "EX a. eval (Pair e1 e2) a"
-    proof auto
-      fix e1'
-      assume "eval e1 e1'"
-      hence "eval (Pair e1 e2) (Pair e1' e2)" by simp
-      thus "EX a. eval (Pair e1 e2) a" by auto
-    qed
-    with False show ?thesis by simp
-  qed
-next case (tprl env e t1 t2)
-  thus ?case
-  proof (cases "is_val e")
-  case True
-    with tprl have "EX e1 e2. e = Pair e1 e2 & typecheck env e1 t1 & typecheck env e2 t2 & is_val e1 & is_val e2" by (simp add: canonical_prod)
-    thus ?thesis
-    proof auto
-      fix e1 e2
-      assume "is_val e1"
-         and "is_val e2"
-      hence "eval (ProjL (Pair e1 e2)) e1" by simp
-      thus "EX a. eval (ProjL (Pair e1 e2)) a" by auto
-    qed
-  next case False
-    with tprl have "EX a. eval e a" by auto
-    thus ?thesis
-    proof auto
-      fix a
-      assume "eval e a"
-      hence "eval (ProjL e) (ProjL a)" by simp
-      thus "EX a. eval (ProjL e) a" by auto
-    qed
-  qed
-next case (tprr env e t1 t2)
-  thus ?case
-  proof (cases "is_val e")
-  case True
-    with tprr have "EX e1 e2. e = Pair e1 e2 & typecheck env e1 t1 & typecheck env e2 t2 & is_val e1 & is_val e2" by (simp add: canonical_prod)
-    thus ?thesis
-    proof auto
-      fix e1 e2
-      assume "is_val e1"
-         and "is_val e2"
-      hence "eval (ProjR (Pair e1 e2)) e2" by simp
-      thus "EX a. eval (ProjR (Pair e1 e2)) a" by auto
-    qed
-  next case False
-    with tprr have "EX a. eval e a" by auto
-    thus ?thesis
-    proof auto
-      fix a
-      assume "eval e a"
-      hence "eval (ProjR e) (ProjR a)" by simp
-      thus "EX a. eval (ProjR e) a" by auto
-    qed
-  qed
-next case (tabt env e t)
-  thus ?case
-  proof (cases "is_val e", auto simp add: canonical_void)
-    fix x
-    assume "eval e x"
-    hence "eval (Abort t e) (Abort t x)" by simp
-    thus "EX x. eval (Abort t e) x" by auto
-  qed
-next case (tinl env e t1 t2)
+next case tc_suc
+  thus ?case by (metis eval_suc is_val.simps(3))
+next case tc_rec
+  thus ?case by (metis eval_rec_1 eval_rec_2 eval_rec_3 is_val.simps(3) canonical_nat)
+next case tc_lam
+  thus ?case by simp
+next case tc_appl
+  thus ?case by (metis eval_appl_1 eval_appl_2 eval_appl_3 canonical_arrow)
+next case tc_triv
+  thus ?case by simp
+next case tc_pair
+  thus ?case by (metis eval_pair_1 eval_pair_2 is_val.simps(10))
+next case tc_projl
+  thus ?case by (metis eval_projl_1 eval_projl_2 canonical_prod)
+next case tc_projr
+  thus ?case by (metis eval_projr_1 eval_projr_2 canonical_prod)
+next case tc_abort
+  thus ?case by (metis eval_abort canonical_void)
+next case tc_case
   thus ?case 
-  proof (cases "is_val e", auto)
-    fix x
-    assume "eval e x"
-    hence "eval (InL t1 t2 e) (InL t1 t2 x)" by simp
-    thus "EX y. eval (InL t1 t2 e) y " by auto
-  qed
-next case (tinr env e t2 t1)
-  thus ?case 
-  proof (cases "is_val e", auto)
-    fix x
-    assume "eval e x"
-    hence "eval (InR t1 t2 e) (InR t1 t2 x)" by simp
-    thus "EX y. eval (InR t1 t2 e) y " by auto
-  qed
-next case (tcse env e t1 t2 el t er)
-  thus ?case
-  proof (cases "is_val e")
-  case True
-    with tcse have "(EX e'. e = InL t1 t2 e' & is_val e' & typecheck env e' t1) | (EX e'. e = InR t1 t2 e' & is_val e' & typecheck env e' t2)" by (simp add: canonical_sum)
-    thus ?thesis
-    proof (cases "EX e'. e = InL t1 t2 e'", auto)
-      fix e'
-      assume "is_val e'" 
-      hence "EX x. eval (Case (InL t1 t2 e') el er) (subst el e')" by simp
-      thus "EX x. eval (Case (InL t1 t2 e') el er) x" by auto
-    next
-      fix e'
-      assume "is_val e'" 
-      hence "EX x. eval (Case (InR t1 t2 e') el er) (subst er e')" by simp
-      thus "EX x. eval (Case (InR t1 t2 e') el er) x" by auto
-    qed
-  next case False
-    with tcse have "EX a. eval e a" by simp
-    thus ?thesis
-    proof auto
-      fix a
-      assume "eval e a"
-      hence "eval (Case e el er) (Case a el er)" by simp
-      thus "EX x. eval (Case e el er) x" by auto
-    qed
-  qed
-next case (tfld env e t)
-  thus ?case
-  proof (cases "is_val e", auto)
-    fix a
-    assume "eval e a"
-    hence "eval (Fold t e) (Fold t a)" by auto
-    thus "EX a. eval (Fold t e) a" by auto
-  qed
-next case (tufd env e t)
-  thus ?case
-  proof (cases "is_val e")
-  case True
-    with tufd have "EX e'. e = Fold t e' & is_val e'" by (simp add: canonical_rec)
-    then obtain e' where E': "e = Fold t e' & is_val e'" by auto
-    hence "eval (Unfold (Fold t e')) e'" by simp
-    hence "EX a. eval (Unfold (Fold t e')) a" by auto
-    with E' show ?thesis by auto
-  next case False
-    with tufd obtain a where "eval e a" by auto
-    hence "eval (Unfold e) (Unfold a)" by auto
-    thus ?thesis by auto
-  qed
-next case ttlm
-  thus ?case by simp
-next case (ttap env e t1 t)
-  thus ?case
-  proof (cases "is_val e")
-  case True
-    with ttap have "EX v. e = TyLam v & typecheck env v t1" by (simp add: canonical_all)
-    then obtain v where V: "e = TyLam v & typecheck env v t1" by auto
-    hence "EX a. eval (TyAp t (TyLam v)) a" by (metis eta1)
-    with V show ?thesis by simp
-  next case False
-    from ttap False obtain a where "eval e a" by auto
-    hence "eval (TyAp t e) (TyAp t a)" by simp
-    thus ?thesis by auto
-  qed
-qed 
+  by (metis eval_case_1 eval_case_2 eval_case_3 is_val.simps(15) is_val.simps(16) canonical_sum)
+next case tc_inl
+  thus ?case by (metis eval_inl is_val.simps(15))
+next case tc_inr
+  thus ?case by (metis eval_inr is_val.simps(16))
+qed
 
 end
